# Tangent Spaces

Lead Question: *What is the velocity of a curve $\gamma$ at point $p$?*


## Velocities 

**Definition**: Let $(\mathcal{M},\mathcal{O},\mathscr{A})$ be a smooth manifold with a curve $\gamma:\mathbb{R}\to\mathcal{M}$ at least $C^1$. Suppose that $\gamma(\lambda_0) = p$. The **velocity** of $\gamma$ at $p$ is the linear map[^1]
\begin{align}
   \mathscr{v}_{\gamma,p}&:C^{\infty}(\mathcal{M})\xrightarrow{\sim}\mathbb{R} \\ 
   f&\mapsto \mathscr{v}_{\gamma, p}(f) := (f\circ \gamma)'(\lambda_0)
\end{align}


[^1]: Where $C^{\infty}(\mathcal{M})$ is the set of smooth functions $f:\mathcal{M}\to\mathbb{R}$ equipped with pointwise addition: $(f+g)(p) = f(p)+g(p)$ and s-multiplication: $(\lambda f)(p) = \lambda f(p)$. 


**Loose idea**: The equivalence with what you've probably seen in the past is that previously we thought of the gradient as $v^i(\partial_i f)$ where $v^i$ is the vector we've dotted into the gradient $\partial_i f$. *All we are doing now* is reinterpretting as $(v^i\partial_i)f$ where the only shift in philosophy is that we now think of the linear map $v^i\partial_i$ acting on the function $f$. Thus, vectors in differential geometry survive as the *directional deriviatves* that they induce. However, if we know how these operators act on *any* function, we may apply them to the coordinate functions in particular to re-obtain our previous notion of the vector components.


## Tangent Vector Space 

**Definition** For each point $p\in\mathcal{M}$, we define the *set* $T_p\mathcal{M}$ as the "tangent space to $\mathcal{M}$ at $p$", i.e. 
\begin{equation}
    T_p\mathcal{M} := \left\{ \mathscr{v}_{\gamma, p} | \gamma \text{ smooth curves through } p \right\}
\end{equation}


Picture: 

![Intrinsic versus extrinsic view of tangent space](/figures/lecture5/intrinsic_extrinsic.png){#fig-intrinsic_extrinsic}


In @fig-intrinsic_extrinsic we see two differing realizations of the tangent space. On the left, we show the tangent space as defined above from an intrinsic standpoint. On the right we see the manifold M embedded in a $d+1$ dimensional space so that $T_p\mathcal{M}$ is a *literal plane*. While these views are technically equivalent, we choose the intrinsic view to be *aesthetically superior*.

**Key observation:** $T_p\mathcal{M}$ can be equipped with a vector space structure. Immediately, we can add two elements from $T_p\mathcal{M}$ pointwise: 
\begin{align}
    +&:T_p\mathcal{M}\times T_p\mathcal{M} \to  \text{Hom}(C^{\infty}(\mathcal{M}), \mathbb{R})\\ 
    (\mathscr{v}_{\gamma, p} + \mathscr{v}_{\delta, p})(f) &:= \mathscr{v}_{\gamma, p}(f) +_{\mathbb{R}} \mathscr{v}_{\delta, p}(f)
\end{align}
and likewise for s-multiplication. It remains to be shown that

1. there actually exists a curve $\sigma$ such that $\mathscr{v}_{\gamma, p} + \mathscr{v}_{\delta, p} = \mathscr{v}_{\sigma, p}$
2. there actually exists a curve $\tau$ such that $\alpha \mathscr{v}_{\gamma, p} = \mathscr{v}_{\tau, p}$

In other words, that we actually end up back in $T_p\mathcal{M}$. Let's start with the proof for s-multiplication: 

Let $\tau: \mathbb{R}\to\mathcal{M}$ be defined such that 
\begin{equation}
    \lambda \mapsto \tau(\lambda) := \gamma(\alpha\lambda + \lambda_0) = (\gamma \circ \mu_\alpha)(\lambda_0)
\end{equation}
where 
\begin{align}
    \mu_\alpha&: \mathbb{R} \to \mathbb{R} \\ 
    r &\mapsto \alpha r + \lambda_0
\end{align}


We see that
\begin{align}
    \tau(0) &= \gamma(\alpha 0 + \lambda_0) = \gamma(\lambda_0) \\ 
    \mathscr{v}_{\tau, p} &= (f\circ \tau)'(0) \\ 
    &= (f\circ \gamma \circ \mu_\alpha)'(0) \\ 
    &= (f\circ \gamma)'(\lambda_0)\cdot \alpha \\ 
    &= \alpha \mathscr{v}_{\gamma, p}
\end{align}
where in the last line we used the chain rule.

Next, let's try out the sum: 
\begin{align}
    \mathscr{v}_{\gamma, p} + \mathscr{v}_{\delta, p} &= \mathscr{v}_{\sigma, p}
\end{align}
We make a choice of chart $(\mathcal{U}, x)$[^1] so that 
\begin{align}
    \sigma&:\mathbb{R} \to \mathcal{M} \\
    \sigma(\lambda)  &:= x^{-1}\Big( (x\circ \gamma)(\lambda_0+\lambda) + (x\circ\delta)(\lambda_1 + \lambda) - (x\circ\gamma)(\lambda_0) \Big)
\end{align}

[^1]: Your *ill-definition* alarm bells should be ringing. In the end, there should be no dependence on the choice of chart of we've done something wrong.


We claim that this does the trick. First, let's look at $\sigma(0)$. We have 
\begin{align}
    \sigma(0) &= x^{-1}\Big( (x\circ\gamma)(\lambda_0) + (x\circ\delta)(\lambda_1) - (x\circ\gamma)(\lambda_0)\Big) \\ 
    &= x^{-1}((x\circ\delta)(\lambda_1)) \\ 
    &= \delta(p)
\end{align}

so we confirmed that we hit the correct point. Now, let's check that the velocity is correct: 
\begin{align}
    \mathscr{v}_{\sigma, p}(f) &= (f\circ\sigma)'(0) \\ 
    &= (f\circ x^{-1} \circ x \circ \sigma)'(0) \\ 
    &= (x^i\circ\sigma)'(0)\partial_i(f\circ x^{-1})(x(\sigma(0))) \\ 
    &= (x^i\circ\sigma)'(0)\partial_i(f\circ x^{-1})(x(p)) \\ 
    &= \Big[ (x^i\circ \gamma)'(\lambda_0)+ (x^i\circ\delta)'(\lambda_1)\Big]\partial_i(f\circ x^{-1})(x(p)) \\ 
    &= (x^i\circ \gamma)'(\lambda_0)\partial_i(f\circ x^{-1})(x(p)) \\ 
    &\qquad + (x^i\circ\delta)'(\lambda_1)\partial_i(f\circ x^{-1})(x(p))  \\ 
    &= (f\circ\gamma)'(\lambda_0) + (f\circ\delta)'(\lambda_1) \\ 
    &= \mathscr{v}_{\gamma, p}(f) + \mathscr{v}_{\delta, p}(f)
\end{align} 

Now we can confirm that the addition and s-multiplication on $T_p\mathcal{M}$ do close thus proving that $T_p\mathcal{M}$ is, in fact, a vector space.


## Components of a Vector with respect to a Chart

**Definition**: Let $(\mathcal{U}, x)\in \mathscr{A}$. Let $\gamma:\mathbb{R}\to\mathcal{M}$ be a curve with $\gamma(0)=p$. Then [^2]
\begin{align}
    \mathscr{v}_{\gamma, p}(f) &= (f\circ \gamma)'(0) \\ 
        &= (f\circ x^{-1} \circ x \circ \gamma)'(0) \\ 
        &= (x^i\circ\gamma)'(0)\partial_i(f\circ x^{-1})(x(p))
\end{align}

[^2]: This formula appears frequently enough that it's worth memorizing.

Because the term is very cumbersome, we use the *notation*
\begin{equation}
    \partial_i(f\circ x^{-1})(x(p)) =: \left[\frac{\partial f}{\partial x^i}\right]_p
\end{equation}
This is **not** a standard partial derivative, *but behaves the same*. Note that $f:\mathcal{M}\to\mathbb{R}$ is a function of the manifold for which we don't have a notion of the *partial derivative*.

The first piece, we may rewrite as 
\begin{equation}
    (x^i\circ \gamma)(0) =: \dot\gamma_x^i(0) 
\end{equation}
so that 
\begin{equation}
    \mathscr{v}_{\gamma, p}(f) = \dot\gamma_x^i(0)\left( \frac{\partial}{\partial x^i}\right)_p f
\end{equation}
Since this is true for all $f\in C^{\infty}(\mathcal{M})$ then in a chart we may understand this as the velocity vector 
\begin{equation}
    \vartheta_{\gamma, p} := \dot\gamma_x^i(0)\left(\frac{\partial}{\partial x^i}\right)_p
\end{equation}

where we think of $\left(\dfrac{\partial}{\partial x^i}\right)_p$ as the *chart-induced-basis* of $T_p\mathcal{M}$.


## Chart-Induced Basis

**Definition**: If $(\mathcal{U}, x)\in\mathscr{A}$, then 
\begin{equation}
    \left(\frac{\partial}{\partial x^1} \right)_p, \left(\frac{\partial}{\partial x^2} \right)_p, ..., \left(\frac{\partial}{\partial x^d} \right)_p, \in T_p\mathcal{M}
\end{equation}
constitute a basis for $T_p\mathcal{U}$. 

To show linear independence, we apply the ith vector to the jth component function

\begin{align}
    0 = \lambda^i\frac{\partial}{\partial x^i} (x^j) 
    &= \lambda^i\partial_i(x^j\circ x^{-1})(x(p)) \\ 
    &= \lambda^i \delta^j_i \\ 
    &= \lambda^j
\end{align}
Thus, these really do constitute a basis.

A corollary of this is that the dimension of $T_p\mathcal{M}$ is $\text{dim}(\mathcal{M})$.



## Change of Cector Components under a Change of Chart

**NOTE**: A tangent vector does not change because *you* decide to use a different chart. The components change. 

**Terminology**: We will now write $X\in T_p\mathcal{M}$ instead of the more cumbersome curve notation. We also may write 
\begin{equation}
    X = X^i\left(\frac{\partial}{\partial x^i} \right)_p
\end{equation}


Let $(\mathcal{U}, x)$, $(\mathcal{V}, y)$ be overlapping charts with $p\in\mathcal{U}\cap\mathcal{V}$. Let $X\in T_p\mathcal{M}$. Then 
\begin{align}
    X &= X_{(x)}^i \left(\frac{\partial}{\partial x^i}\right)  = X_{(y)}^i\left(\frac{\partial}{\partial y^i}\right)_p\\ 
\end{align}
consider the following: 
\begin{align}
    \frac{\partial}{\partial x^i}f &= \partial_i(f\circ x^{-1})(x(p)) \\ 
        &= \partial_i \left( f \circ y^{-1} \circ y \circ x^{-1}\right)(x(p)) \\ 
        &= \partial_i(y^j \circ x^{-1})(x(p)) \cdot \partial_j(f\circ y^{-1})(y(p)) \\
        &= \frac{\partial y^j}{\partial x^i}\cdot \frac{\partial f}{\partial y^j} \\
        &= \left(\frac{\partial y^j}{\partial x^i}\right)\cdot \left(\frac{\partial }{\partial y^j}\right) f\\
\end{align}

Therefore, insertion into the previous equation yields 
\begin{align}
    X_{x}^i \frac{\partial y^j}{\partial x^i}\frac{\partial}{\partial y^j}  &= X_{(y)}^j\frac{\partial}{\partial y^j} \\ 
    X_{(y)}^j &= \left(\frac{\partial y^j}{\partial x^i} \right) X_{(x)}^i
\end{align}
which is exactly the transformation law for the components of a tangent vector $X$ when we switch between two charts with coordinate functions $x^i$ and $y^j$.



## Cotangent Spaces 
Given that we have $T_p\mathcal{M}$, it is natural to consider $(T_p\mathcal{M})^*$, i.e. the dual to the tangent space: 
\begin{equation}
    (T_p\mathcal{M})^* := \left\{\phi: T_p\mathcal{M}\xrightarrow{\sim} \mathbb{R} \right\}
\end{equation}

**Example**: Consider $f\in C^{\infty}(\mathcal{M})$. Then 
\begin{align}
    (df)_p &:  T_p\mathcal{M} \xrightarrow{\sim} \mathbb{R} \\ 
      X &\mapsto (df)_p(X) := Xf
\end{align}

i.e. $(df)_p\in(T_p\mathcal{M})^*$! This is called the gradient of $f$ at $p\in\mathcal{M}$.

Further, we can calculate the components of the gradient... 
\begin{align}
    \left((df)_p\right)_j &:= (df)_p \left(\frac{\partial }{\partial x_j}\right)_p \\ 
    &= \left( \frac{\partial f}{\partial x^j} \right)_p
\end{align}

Upshot: The gradient of a function *is not a vector*, it's a covector!



**Theorem**: Consider the chart $(\mathcal{U}, x)$ so that we have coordinate maps $x^i:\mathcal{U}\to\mathbb{R}$. The claim is 
\begin{equation}
    (d x^1)_p, (d x^2)_p, ..., (d x^d)_p
\end{equation}
is the *dual basis* for $T_p^*\mathcal{M}$. Observe: 
\begin{align}
    (d x^a)_p(\frac{\partial }{\partial x^b}) = \frac{\partial x^a}{\partial x^b} = \delta_b^a
\end{align}


## Change of components of a covector with respect to a change of chart. 

Let $\omega \in T_p^*\mathcal{M}$, then 
\begin{align}
    \omega_{(y)j}(dy^j)_p &= \omega = \omega_{(x)i} (dx^i)_p \\ 
    \Rightarrow \omega_{(y)i} &= \frac{\partial x^j}{\partial y^i}\omega_{(x)j}
\end{align}
[^3]

[^3]: In the tutorial session, we will show that $\frac{\partial x^i}{\partial y^j}$ is the matrix inverse to $\frac{\partial y^m}{\partial x^n}$
